SP1Foundations/Assumptions.lean
@@ -70,7 +70,7 @@ namespace Opcode
       ∧ (imm_c = 1 → shift_i_type_constraints op_a op_b_0 op_b_1 op_b_2 op_b_3 op_c_0 op_c_1 op_c_2 op_c_3 imm_b imm_c)
   | LUI | AUIPC =>
       (imm_b = 1 ∧ imm_c = 1)
-      ∧ op_b_0 >= 2^12
+      ∧ op_b_0.val % 2 ^ 12 = 0
       ∧ BitVec.signExtend 64 (BitVec.ofNat 32 (op_b_0.val + op_b_1.val * 65536)) = Word.toBitVec64 #v[op_b_0, op_b_1, op_b_2, op_b_3]
   | JAL =>
       (imm_b = 1 ∧ imm_c = 1) ∧
